working in the cycle

dafny/cycle.dfy
@@ -1,4 +1,5 @@
 include "modDiv.dfy"
+include "list.dfy"
 
 /**
  * Define the cycle function
@@ -9,66 +10,68 @@ include "modDiv.dfy"
  */
 module Cycle {
 
+    import List
     import ModDiv
 
     function method isCycle(list: seq<nat>, listCycle: seq<nat>): bool
         requires |list| > 0;
     {
-        var equalsMod := forall k : nat :: 0 <= k < |listCycle| ==> listCycle[k] == list[ ModDiv.mod(k, |list|) ];
+        var upperLimit := if |list| < |listCycle| then |list| else |listCycle|;
 
-        equalsMod
+        var equalFirst     := forall k : nat :: 0      <= k < upperLimit           ==> listCycle[k] == list[k];
+        var equalsPrevious := forall k : nat :: |list| <= k < |listCycle|          ==> listCycle[k] == listCycle[k - |list|];
+        var equalsNext     := forall k : nat :: 0      <= k < |listCycle| - |list| ==> listCycle[k] == listCycle[k + |list|];
+
+        equalFirst && equalsPrevious && equalsNext
     }
-    function method isCycleGap(list: seq<nat>, listCycle: seq<nat>, gap: nat): bool
-        requires |list| > 0;
-    {
-        var equalsMod := forall k : nat :: 0 <= k < |listCycle| ==> listCycle[k] == list[ ModDiv.mod(k + gap, |list|) ];
-
-        equalsMod
-    }
-
-    function method cyclePos(list: seq<nat>, pos: nat): nat
-        requires |list| > 0;
-        ensures cyclePos(list,pos) == list[ModDiv.mod(pos,|list|)];
-    {
-        var l := |list|;
-        var k := ModDiv.mod(pos, l);
-        assert k < l;
-        var result := list[k];
-        result
-    }
-
-    method cycle(source: seq<nat>, size: nat) returns (result: seq<nat>)
+ 
+    function method cyclePos(source: seq<nat>, pos: nat): nat
         requires |source| > 0;
-        ensures forall k : nat :: 0 <= k < |result| ==> ModDiv.mod(k,|source|) < |source|;
-        ensures forall k : nat :: 0 <= k < |result| ==> result[k] == source[ModDiv.mod(k,|source|)];
-        ensures |result| == size;
+        ensures pos < |source| ==> cyclePos(source,pos) == source[pos];
+        ensures pos > |source| ==> cyclePos(source,pos) == cyclePos(source, pos - |source|);
+        ensures cyclePos(source,pos) == if pos < |source| then source[pos] else cyclePos(source, pos - |source|)
+        decreases pos;
     {
-        result := [];   
-        while( |result| < size ) 
-            invariant forall k : nat :: 0 <= k < |result| ==> result[k] == source[ModDiv.mod(k,|source|)];
-            invariant |result| <= size;
-            decreases size - |result|;
-        {
-            var value := cyclePos(source, |result|);
-            result := result + [value];
-        }
-        assert |result| == size;
-    }    
+        var s := |source|;
+        assert s > 0;
+        assert s > 0 ==> pos - s < pos;
+
+        var cyclePosResult := if pos < |source| then source[pos] else cyclePos(source, pos - |source|);
+
+        var posPlusSource := pos + |source|;
+
+        cyclePosResult
+    }
+ 
+    function method cycle(source: seq<nat>, size: nat): seq<nat>
+        requires |source| > 0;
+        ensures |cycle(source,size)| == size;
+        ensures isCycle(source, cycle(source,size));
+        decreases size;
+    {
+        var cycleList := if size == 0 then [] else
+        cycle(source,size-1) + [cyclePos(source,size - 1)];
+
+        assert |cycleList| == size;
+        assert |cycleList| > 0 ==> cycleList[0] == cyclePos(source,0);
+        
+        assert forall k: nat {:induction k} :: 0 <= k < |cycleList| ==> cycleList[k] == cyclePos(source,k);
+
+        cycleList
+    }
 
     /**
-     * Since the current definition of the cycle mod is alligned with the definition of the isModDiv
-     * all the properties defined to the isModDiv can be applied to the cycle.
+     * Ensure that the ModList is Cycle
      */
-    lemma cycleIsMod(list: seq<nat>, listCycle: seq<nat>, m: nat)
-        requires |list| > 0;
-        requires |listCycle| == |list| * m;
-        requires isCycle(list, listCycle);
-        ensures forall k : nat :: 0 <= k < |listCycle| ==> ModDiv.isModDiv(k, |list|, m, ModDiv.mod(k, |list|));
+    lemma modIsCycle(modList: seq<nat>, loopValue: nat)
+        requires loopValue > 0;
+        requires |modList| > 0;
+        requires loopValue <= |modList|;
+        requires ModDiv.isModList(loopValue, modList);
+        ensures isCycle(modList[..loopValue], modList);
     {
-        assert forall k : nat :: 0 <= k < |listCycle| ==> listCycle[k] == list[ ModDiv.mod(k, |list|) ];
-        //  * assert division * b + remainder == a
-        //  * assert remainder < b;
-        //  * assert remainder <= a;
+        ModDiv.modListValuesRepeat(modList, loopValue);
+        var smallList := modList[..loopValue];
     }
 
     lemma cycleShouldContainsList(list: seq<nat>, cycleList: seq<nat>)
@@ -79,26 +82,209 @@ module Cycle {
     {
     }
 
-    lemma cycleByConcat(list: seq<nat>, cycleList: seq<nat>, smallCycle: seq<nat>, m: nat)
+    lemma cycleAlwaysRepeatTheSameValues(list: seq<nat>, listCycle: seq<nat>, m: nat)
+        requires m > 1;
         requires |list| > 0;
-        requires |cycleList| > |list|;
-        requires |smallCycle| > |list|;
-        requires isCycle(list, cycleList);
-        requires isCycle(list, smallCycle);
-        requires |cycleList| == |list| * m;
-        requires |smallCycle| == |cycleList| - |list|;
-        requires |smallCycle| == |list| * ( m - 1 );
-        requires m > 0;
-        ensures cycleList == list + cycleList[|list|..];
-        ensures cycleList == list + smallCycle;
+        requires |listCycle| == |list| * m;        
+        requires isCycle(list, listCycle);
     {
-        assert cycleList[0..|list|] == list;
+        // going up //
+        var k := 0;
+        while ( k < |list| )
+            decreases |list| - k;
+            invariant k <= |list|;
+        {
+            var smallListValue := list[k];
+            var bigKey := k;
+            var n := 0;
+            while ( bigKey < |listCycle| )
+                decreases |listCycle| - bigKey;
+                invariant bigKey == k + n * |list|;
+                invariant ModDiv.mod(k + n * |list|,|list|) == ModDiv.mod(k,|list|);
+                invariant ModDiv.mod(k,|list|) == k;
+                invariant ModDiv.mod(bigKey,|list|) == k;
+                invariant list[k] == list[ModDiv.mod(bigKey,|list|)];
+                invariant bigKey < |listCycle| ==> listCycle[bigKey] == list[k];
+                invariant bigKey < |listCycle| ==> listCycle[bigKey] == list[ModDiv.mod(bigKey,|list|)];
+            {
+                assert smallListValue == listCycle[bigKey];
+                assert bigKey == k + n * |list|;
+                assert smallListValue == listCycle[bigKey];
+                ModDiv.modSmallValues(k,|list|);
+                assert k < |list|;
+                assert ModDiv.mod(k,|list|) == k;
+                ModDiv.modAOnBEqualsModAMoreMTimesB(k,|list|,n);
+                assert ModDiv.mod(k + n * |list|,|list|) == ModDiv.mod(k,|list|);
+                assert ModDiv.mod(bigKey,|list|) == ModDiv.mod(k,|list|);
+                assert ModDiv.mod(bigKey,|list|) == k;
+                if ( bigKey + |list| < |listCycle| )
+                {
+                    assert listCycle[bigKey] == listCycle[bigKey + |list|];
+                }
+                n := n + 1;
+                bigKey := bigKey + |list|;
+                ModDiv.modAOnBEqualsModAMoreMTimesB(k,|list|,n);
+                assert ModDiv.mod(k + n * |list|,|list|) == ModDiv.mod(k,|list|);
+                assert ModDiv.mod(bigKey,|list|) == ModDiv.mod(k,|list|);
+            }
+            k := k + 1;
+        }
+        
+        assert forall k : nat :: k <= 0 < |listCycle| ==> listCycle[k] == list[ModDiv.mod(k,|list|)];
     }
 
-//     method Main()
+    // sounds good, does not work
+    //
+    // lemma cycleAlwaysRepeatTheSameValues(list: seq<nat>, listCycle: seq<nat>, m: nat)
+    //     requires m > 1;
+    //     requires |list| > 0;
+    //     requires |listCycle| == |list| * m;        
+    //     requires isCycle(list, listCycle);
+    //     ensures
+    //         forall k : nat :: 0 <= k < |list|   ==> 
+    //         forall n : nat :: 0 <= n < m        ==> 
+    //         k + n * |list| < |listCycle|        ==> 
+    //         listCycle[k + n * |list|] == list[k];
+    // {
+    //     assert forall k : nat :: 0      <= k < |list|      ==> listCycle[k] == list[k];
+    //     assert forall k : nat :: |list| <= k < |listCycle| ==> listCycle[k] == listCycle[k - |list|];
+
+
+    //     // going up //
+    //     var k := 0;
+    //     while ( k < |list| )
+    //         decreases |list| - k;
+    //         invariant k <= |list|;
+    //     {
+    //         var current := list[k];
+    //         var next := k;
+    //         var n := 0;
+    //         assert next == k + n * |list|;
+    //         while ( next < |listCycle| )
+    //             decreases |listCycle| - next;
+    //             invariant next < |listCycle| ==> current == listCycle[next];
+    //             invariant next < |listCycle| ==> current == list[k];
+    //             invariant next < |listCycle| ==> listCycle[next] == list[k];
+    //             invariant next == k + n * |list|;
+    //             invariant next < |listCycle| ==> listCycle[k + n * |list|] == list[k];
+    //             invariant 
+    //                 k + n * |list| < |listCycle|        ==> 
+    //                 listCycle[k + n * |list|] == list[k];
+    //         {
+    //             assert current == listCycle[next];
+    //             assert next == k + n * |list|;
+    //             assert listCycle[k + n * |list|] == list[k];
+    //             n := n + 1;
+    //             next := next + |list|;
+    //         }
+    //         assert next >= |listCycle|;
+    //         k := k + 1;
+    //     }
+    //     assert k == |list|;
+
+    //     // going down //
+    //     k := 0;
+    //     while ( k < |listCycle| )
+    //         decreases |listCycle| - k;
+    //         invariant k <= |listCycle|;
+    //     {
+    //         var current := listCycle[k];
+    //         var prev := k;
+    //         var n := 0;
+    //         assert prev == k - n * |list|;
+    //         while ( prev > |list| )
+    //             decreases prev;
+    //             invariant prev >= 0 ==> current == listCycle[prev];
+    //             invariant prev >= |list| ==> current == listCycle[prev - |list|];
+    //             invariant prev == k - n * |list|;
+    //             // invariant 
+    //             //     k + n * |list| < |listCycle|        ==> 
+    //             //     listCycle[k + n * |list|] == list[k];
+    //         {
+    //             assert current == listCycle[prev];
+    //             assert listCycle[prev] == listCycle[prev - |list|];
+    //             assert prev == k - n * |list|;
+    //             assert listCycle[k - n * |list|] == listCycle[prev - |list|];
+    //             n := n + 1;
+    //             prev := prev - |list|;
+    //         }
+    //         assert prev <= |list|;
+    //         k := k + 1;
+    //     }
+
+    //     assert
+    //         forall k : nat :: 0 <= k < |list|   ==> 
+    //         forall n : nat :: 0 <= n < m        ==> 
+    //         k + n * |list| < |listCycle|        ==> 
+    //         listCycle[k + n * |list|] == list[k];
+    // }
+
+    // lemma cycleByConcat(list: seq<nat>, cycleList: seq<nat>, smallCycle: seq<nat>, m: nat)
+    //     requires |list| > 0;
+    //     requires |cycleList| > |list|;
+    //     requires |smallCycle| > |list|;
+    //     requires isCycle(list, cycleList);
+    //     requires isCycle(list, smallCycle);
+    //     requires |cycleList| == |list| * m;
+    //     requires |smallCycle| == |cycleList| - |list|;
+    //     requires |smallCycle| == |list| * ( m - 1 );
+    //     requires m > 0;
+    //     ensures cycleList == list + cycleList[|list|..];
+    //     ensures smallCycle == cycleList[..|smallCycle|];
+    //     ensures cycleList == list + smallCycle;
+    // {
+    //     assert smallCycle[0..|list|] == list;
+    //     assert cycleList[0..|list|] == list;
+    //     assert forall k: nat 
+    // }
+
+
+//     lemma sumMultipleList(list: seq<nat>, cycleList: seq<nat>, m: nat)
+//         requires m > 0;
+//         requires |list| > 0;
+//         requires |cycleList| > 0;
+//         requires |cycleList| >= |list|;
+//         requires isCycle(list, cycleList);
+//         requires |cycleList| == |list| * m;
+//         ensures List.sum(cycleList) == List.sum(list) * m;
+//         decreases cycleList, m;
 //     {
-//         print("\ntesting cycle\n");
-//         print(isCycle([1,2,3],[1,2,3,1,2,3,1,4]));
-//         print("\n:D\n");
+//         if m == 1 {
+//             assert cycleList == list;
+//         } else {
+//             var smallCycle := cycleList[|list|..];
+//             assert cycleList == list + smallCycle;
+//             assert isCycle(list, smallCycle);
+//             List.distributiveSum(list,smallCycle);
+//             assert List.sum(cycleList) == List.sum(list) + List.sum(smallCycle);
+//             sumMultipleList(list,smallCycle, m-1);
+//         }
 //     }
+
+//     lemma cycleListIsListPlusSmallCycleList(list: seq<nat>, cycleList: seq<nat>, smallCycle: seq<nat>, m: nat)
+//         requires |list| > 0;
+//         requires |cycleList| >= |list|;
+//         requires m > 0;
+//         requires isCycle(list, cycleList);
+//         requires |cycleList| == |list| * m;
+//         requires smallCycle == cycleList[|list|..];
+//         ensures cycleList == list + smallCycle;
+//         ensures List.sum(cycleList) == List.sum(list) + List.sum(smallCycle);
+//         ensures |smallCycle| > 0 ==> isCycle(list, smallCycle);
+//         ensures |smallCycle| == |list| * (m - 1);
+//     {
+//         List.distributiveSum(list,smallCycle);
+//         assert |cycleList| == |list| * m;
+//         assert forall v : nat :: 0 <= v < |list| ==> cycleList[v] == list[v];
+//         assert |cycleList| >= |list|;
+//         assert cycleList == list + smallCycle;
+//         assert |smallCycle| > 0 ==> isCycle(list,smallCycle);
+//         assert |smallCycle| == |list| * (m - 1);
+//     }
+// //     method Main()
+// //     {
+// //         print("\ntesting cycle\n");
+// //         print(isCycle([1,2,3],[1,2,3,1,2,3,1,4]));
+// //         print("\n:D\n");
+// //     }
 }
