dafny/integral.dfy
@@ -1,0 +1,267 @@
+include "modDiv.dfy"
+include "list.dfy"
+include "cycleFromMod.dfy"
+
+module Integral {
+
+    import ModDiv
+
+    function sorted(list: seq<nat>): bool {
+        forall k : nat :: 1 <= k < |list| ==> list[k] > list[k-1]
+    }
+
+    function nonZero(list: seq<nat>): bool
+    {
+        forall l: nat :: 0 <= l < |list| ==> list[l] > 0
+    }
+
+    function unique(list: seq<nat>): bool {
+        forall n,m : nat :: 0 <= n < m < |list| ==> list[n] != list[m]
+    }
+
+    function first(list: seq<nat>): nat 
+        requires |list| > 0;
+    {
+        list[0]
+    }
+
+    function last(list: seq<nat>): nat 
+        requires |list| > 0;
+    {
+        list[|list|-1]
+    }
+
+    function method sum(list: seq<nat>): nat
+        decreases |list|;
+    {
+        if (|list| == 0 ) then 0 else
+        list[0] + sum(list[1..])
+    }
+
+
+    ghost method distributiveSum(a: seq<nat>, b: seq<nat> )
+        ensures sum(a + b) == sum(a) + sum(b); 
+    {
+        assert |a| == 0 && |b| == 0 ==> sum(a) + sum(b) == 0 == sum(a + b);
+        assert |a|  > 0 && |b| == 0 ==> a + b == a;    
+        assert |a|  > 0 && |b| == 0 ==> sum(a) + sum(b) == sum(a) + 0 == sum(a) == sum(a + b);
+        assert |a| == 0 && |b|  > 0 ==> a + b == b;
+        assert |a| == 0 && |b|  > 0 ==> sum(a) + sum(b) == sum(b) + 0 == sum(b) == sum( a + b);
+        assert |a|  > 0 && |b|  > 0 ==> sum(a) + sum(b) == a[0] + sum(a[1..]) + b[0] + sum(b[1..]) == a[0] + b[0] + sum(a[1..]) + sum(b[1..]);
+        assert |a|  > 0 && |b|  > 0 ==> a + b == [a[0]] + (a[1..] + b);
+        assert |a|  > 0 && |b|  > 0 ==> sum(a + b) == sum([a[0]]) + sum(a[1..] + b);
+    }
+
+    lemma divSum(list: seq<nat>, n: nat)
+        requires 0 <= n < |list|;
+        ensures sum(list) == sum(list[0..n]) + sum(list[n..]); 
+    {
+        assert list[0..n] + list[n..] == list;
+        var a := list[0..n];
+        var b := list[n..];
+        distributiveSum(a,b);
+    }
+
+    lemma sumListPlusValue(list: seq<nat>, value: nat)
+        ensures sum(list) + value == sum([value] + list);
+        ensures sum(list) + value == sum(list + [value]);
+        ensures value + sum(list) == sum(list) + value;
+    {
+        assert sum(list) + value == sum([value] + list);
+        var a := list;
+        var b := [value];
+        distributiveSum(a, b);
+    }
+
+    lemma cycleListIsListPlusSmallCycleList(list: seq<nat>, cycleList: seq<nat>, smallCycle: seq<nat>, m: nat)
+        requires |list| > 0;
+        requires |cycleList| >= |list|;
+        requires m > 0;
+        requires isCycle(list, cycleList);
+        requires |cycleList| == |list| * m;
+        requires  smallCycle == cycleList[|list|..];
+        ensures cycleList == list + smallCycle;
+        ensures sum(cycleList) == sum(list) + sum(smallCycle);
+        ensures |smallCycle| > 0 ==> isCycle(list, smallCycle);
+        ensures |smallCycle| == |list| * (m - 1);
+    {
+        distributiveSum(list,smallCycle);
+        assert |cycleList| == |list| * m;
+        assert forall v : nat :: 0 <= v < |list| ==> cycleList[v] == list[v];
+        assert |cycleList| >= |list|;
+        assert cycleList == list + smallCycle;
+        assert |smallCycle| > 0 ==> isCycle(list,smallCycle);
+        assert |smallCycle| == |list| * (m - 1);
+    }
+
+    function isIntegral(list: seq<nat>, initial: nat, listIntegral: seq<nat>): bool
+        requires |list| == |listIntegral|;
+    {
+        forall v: nat :: 0 <= v < |list| ==> listIntegral[v] == sum(list[0..v+1]) + initial
+    }
+
+    method integral(list: seq<nat>, initial: nat ) returns (result: seq<nat>)
+        ensures |list| == |result|;
+        ensures isIntegral(list,initial,result);
+    {
+        var distance := |list|;
+        var arr := new nat[distance];
+        var k := 0;
+        var acc := initial;
+        while (k < |list|)
+            decreases |list| - k;
+            invariant 0 <= k <= |list|;
+            invariant forall v: nat :: 0 <= v < k ==> arr[v] == sum(list[..v+1]) + initial;
+        {
+            /* 
+             * Could not make it work using acc, what would be fast.
+             * This is not the fast strategy, but for sure is correct
+             */
+            arr[k] := sum(list[..k+1]) + initial;
+            k := k + 1;
+        }
+        // array to seq
+        result := arr[..];
+    }
+
+    function isModList(list: seq<nat>, value: nat, modList: seq<nat>): bool
+    requires |list| == |modList|;
+    requires |list| > 0;
+    requires value > 0;
+    {
+        forall v: nat :: 0 <= v < |list| ==> modList[v] == ModDiv.mod(list[v], value)
+    }
+
+    function isNotMultiple(list: seq<nat>, value: nat): bool
+    requires value > 0;
+    requires |list| > 0;
+    {
+        forall v: nat :: 0 <= v < |list| ==> ModDiv.mod(list[v], value) != 0
+    }
+
+    lemma modOfIntegral(
+        list: seq<nat>, 
+        initial: nat, 
+        integralList: seq<nat>, 
+        modIntegralList: seq<nat>, 
+        m: nat, 
+        cycleList: seq<nat>, 
+        integralCycle: seq<nat>,
+        modIntegralCycle: seq<nat>
+    )
+
+    // m is bigger than zero
+    requires m > 0;
+
+    // list is non zero, non empty and the sum of the list is multiple of m
+    requires |list| > 0;
+    requires nonZero(list);
+    requires ModDiv.mod(sum(list),m) == 0;
+
+
+    // integral list def
+    requires |integralList| == |list|;
+    requires isIntegral(list, initial, integralList);
+    
+    // mod of integral list def
+    requires |modIntegralList| == |integralList|;
+    requires isModList(integralList, m, modIntegralList);
+
+    // cylce list def
+    requires |cycleList| == |list| * m;
+    requires |cycleList| >= |list|;
+    requires isCycle(list, cycleList)
+
+    // integral cycle def
+    requires |integralCycle| == |cycleList|;
+    requires isIntegral(cycleList, initial, integralCycle);
+    
+    // mod of integral cycle def
+    requires |modIntegralCycle| == |integralCycle|;
+    requires isModList(integralCycle, m, modIntegralCycle);
+
+    // mod of integral should be cycle
+//    ensures isCycle(modIntegralList, modIntegralCycle);
+    {
+        if ( m == 1 ) {
+            assert cycleList == list;
+            assert integralCycle == integralList;
+            assert modIntegralCycle == modIntegralList;
+        } else {
+            assert cycleList[0..|list|] == list;
+
+            assert forall v: nat :: 0 <= v < |integralList| ==> integralList[v] == sum(list[..v+1]) + initial;
+            var last := |list| - 1;
+            assert integralList[last] == sum(list[..(last+1)]) + initial;
+            assert list[..(last+1)] == list;
+            assert sum(list[..(last+1)]) == sum(list);
+            assert integralList[last] == sum(list) + initial;
+            assert ModDiv.mod(sum(list),m) == 0;
+            
+        }
+    }
+
+    // lemma bigProoff(
+    //     initial: nat,  // 5
+    //     prev: seq<nat>, // [ 2 3 ]
+    //     list: seq<nat>, // [ 2 4 ]
+    //     integralList: seq<nat>, // [ 7 11 ]
+    //     modList: seq<nat>, // [2, 1]
+    //     modIntegralList: seq<nat>, // [1, 2]
+    //     m: nat, // 3
+    //     cycleList: seq<nat>, // [ 2 4 2 4 2 4 ]
+    //     integralCycle: seq<nat>, // [ 7 11 13 17 19 23 ]
+    //     modIntegralCycle: seq<nat> // [ 1 2 1 2 1 2 ]
+    // )
+    //     requires m > 0;
+    //     requires |list| > 0;
+    //     requires nonZero(list);
+    //     requires |cycleList| == |list| * m;
+    //     requires |list| == |integralList|;
+
+    //     requires |modList| == |list|;
+    //     requires isModList(list, m, modList);
+    //     requires nonZero(modList);
+
+    //     requires isIntegral(list, initial, integralList);
+    //     requires isCycle(list, cycleList);
+    //     requires |integralCycle| == |cycleList|;
+    //     requires isIntegral(cycleList, initial, integralCycle);
+
+    //     // // if the list integral is not multiple of m
+    //     requires isNotMultiple(integralList, m);
+    //     requires |modIntegralList| == |integralList|;
+    //     requires isModList(integralList, m, modIntegralList);
+    //     requires nonZero(modIntegralList);
+
+    //     requires |modIntegralCycle| == |integralCycle|;
+    //     requires isModList(integralCycle, m, modIntegralCycle);
+
+    //     requires ModDiv.mod(sum(list), m) == 0; // [2 4] ==> 2 + 4 == 6 ==> 6 % 3 == 0;
+        
+    //     // the next integral should also be not multiple of m
+    //     ensures isNotMultiple(integralCycle, m);
+    //     ensures nonZero(modIntegralCycle);
+    // {
+    // }
+
+    method testIntegral(v:nat, list: seq<nat>, initial: nat)
+    {
+        var a := [1,2,3];
+        assert a[..1] == [a[0]];
+ 
+        var empty := integral([], initial);
+        assert  empty == [];
+ 
+        var single := [v];
+        var singleIntegral := integral(single, initial);
+        assert singleIntegral[0] == sum(single[..1]) + initial;
+
+        var listIntegral := integral(list, initial);
+        assert forall n: nat ::  0 < n < |list| ==> listIntegral[n] == sum(list[..n+1]) + initial;
+        assert |listIntegral| == |list|;
+    }
+
+    method Main() {
+    }
+}
